lean4/Automaton/NFA/Basic.lean
@@ -1,6 +1,8 @@
 import Mathlib.Data.Set.Lattice
 import Automaton.Language.Basic
 import Automaton.Finset.Basic
+import Mathlib.Data.Finset.Powerset
+import Mathlib.Data.FinEnum
 
 /-!
   This file contains the definition of NFA as well as a few fundemantal operations
@@ -9,29 +11,30 @@ import Automaton.Finset.Basic
 
 namespace NFA
 
-structure NFA (α : Type _)(σ : Type _) where
-  q : Finset α        -- states
-  init : α          -- initial state
-  fs : Finset α       -- accepting states
-  δ : α → σ → Finset α -- transition function
-  [dec : DecidableEq α]
+structure NFA (σ : Type _) where
+  q : Type _             -- states
+  init : q               -- initial state
+  fs : Finset q          -- accepting states
+  δ : q → σ → Finset q   -- transition function
+  [fn : FinEnum q]
 
-variable {α : Type _}{σ : Type _} [DecidableEq α] (t : NFA α σ)
+variable {α : Type _}{σ : Type _} [DecidableEq α] (t : NFA σ)
 
+instance : FinEnum t.q := t.fn
 
 -- one step in the operation of NFA, consuming one character
 -- take the union of all sets of states reachable from current set of states
-def δ_step  (q : Finset α) (e : σ) : Finset α := q.biUnion (fun n => t.δ n e)
+def δ_step  (q : Finset t.q) (e : σ) : Finset t.q := q.biUnion (fun n => t.δ n e)
 
 -- δ* function for NFA
 -- returns set of states reached after inputting a word
-def δ_star : (w : word σ) → Finset α
+def δ_star : (w : word σ) → Finset t.q
   | [] => {t.init}
   | e :: es => δ_step t (δ_star es) e 
 
 -- Whether a word is in the language that the NFA accepts
 def nfa_accepts (w : word σ) : Prop := by
-  have inter : Finset α := (δ_star t w) ∩ t.fs
+  have inter : Finset t.q := (δ_star t w) ∩ t.fs
   exact inter.Nonempty
 
 -- nfa accepts nil iff init is final
@@ -45,5 +48,6 @@ theorem nfa_accepts_nil_iff_final : nfa_accepts t [] ↔ t.init ∈ t.fs := by
     dsimp [nfa_accepts,δ_star]
     rw [Finset.singleton_inter_of_mem e]
     exact (Finset.singleton_nonempty t.init)
+
 
 end NFA
