lean4/Automaton/NFA/ToDFA.lean
@@ -2,23 +2,66 @@ import Automaton.NFA.Basic
 import Automaton.DFA.Basic
 import Mathlib.Data.Finset.Powerset
 
+/-!
+  This file contains conversion from NFA to DFA `nfa_to_dfa`
+  Proves several things about such converted automata such as equality of δ_star function
+  Then asserts that the converted DFA fulfills this property
+-/
+
 open NFA DFA
 
 namespace ToDFA
 
-variable {α : Type _}{σ : Type _} [DecidableEq α] (tn : NFA α σ)
+variable {α : Type _}{σ : Type _} [DecidableEq α] (tn : NFA σ)
 
--- turn nfa function into dfa
-def nfa_δ_to_dfa_δ : Finset α → σ → Finset α := by
+@[simp]
+def nfa_to_dfa_q : Finset (Finset tn.q) := by
+  have qs : Finset tn.q := ⟨ Multiset.ofList (FinEnum.toList tn.q) , by apply FinEnum.nodup_toList⟩
+  exact qs.powerset
+
+@[simp]
+def nfa_to_dfa_init : { x // x ∈ nfa_to_dfa_q tn } := ⟨{tn.init} , by simp [nfa_to_dfa_q]⟩ 
+
+@[simp]
+theorem all_in_q (q : Finset tn.q) : q ∈ nfa_to_dfa_q tn := by
+  simp [nfa_to_dfa_q, · ⊆ ·]
+
+@[simp]
+def nfa_to_dfa_fs : Finset { x // x ∈ nfa_to_dfa_q tn } := by
+  have fs := (nfa_to_dfa_q tn).filter (fun q => (q ∩ tn.fs).Nonempty)
+  apply fs.biUnion
+  intro q
+  exact {⟨q , all_in_q tn q⟩}
+  
+def nfa_to_dfa_δ : { x // x ∈ nfa_to_dfa_q tn } → σ → { x // x ∈ nfa_to_dfa_q tn } := by
   intro q e
-  exact q.biUnion (fun n => tn.δ n e)
+  have q₁ : Finset tn.q := q.1.biUnion (fun q => tn.δ q e)
+  exact ⟨q₁ , all_in_q tn q₁⟩
 
--- δ_star for converted dfa
-def δ_star (w : word σ) : Finset (Finset α) := by
+def nfa_to_dfa : DFA σ := 
+  {q := nfa_to_dfa_q tn, init := nfa_to_dfa_init tn, fs := nfa_to_dfa_fs tn , δ := nfa_to_dfa_δ tn} 
+
+
+theorem δ_star_eq : ⟨(NFA.δ_star tn w) , all_in_q tn (NFA.δ_star tn w)⟩ = (DFA.δ_star (nfa_to_dfa tn) w) := by
   induction w with
-  | nil => exact {{tn.init}}
-  | cons e _ s => exact s.biUnion (fun n => {(nfa_δ_to_dfa_δ tn) n e})
+  | nil => simp [NFA.δ_star,DFA.δ_star,nfa_to_dfa]
+  | cons a as s => simp [NFA.δ_star,DFA.δ_star]
+                   rw [←s]
+                   simp [nfa_to_dfa,nfa_to_dfa_δ,δ_step]
+  
+theorem nfa_to_dfa_eq (w : word σ) : nfa_accepts tn w ↔ dfa_accepts (nfa_to_dfa tn) w := by
+  apply Iff.intro
+  · simp [nfa_accepts,dfa_accepts]
+    intro a
+    rw [←δ_star_eq]
+    simp [nfa_to_dfa]
+    apply And.intro
+    · simp [·⊆·]
+    · exact a
+  · simp [nfa_accepts,dfa_accepts]
+    intro a
+    rw [←δ_star_eq] at a
+    simp [nfa_to_dfa] at a
+    exact a.2
 
--- the final state are all sets of states that include at least one final state
-def fs : Finset (Finset α) := by
-  exact (Finset.powerset tn.q).filter (fun q => (q ∩ tn.fs).Nonempty) 
+end ToDFA
