lean4/Automaton/DFA/ToNFA.lean
@@ -6,24 +6,24 @@ import Automaton.Finset.Basic
   This file contains conversion from DFA to NFA `dfa_to_nfa`
   Proves several things about such converted automata such as equality of δ_star function
   Contains a definition of what equality between NFA and DFA means
-  Then asserts that the converted DFA fulfills is property
+  Then asserts that the converted DFA fulfills this property
 -/
 
 open DFA NFA
 
 namespace ToNFA
 
-variable {α : Type _} {σ : Type _} [DecidableEq α] (td sd : DFA α σ) (tn sn : NFA α σ)
+variable {α : Type _} {σ : Type _} [DecidableEq α] (td sd : DFA σ) (tn sn : NFA σ)
 
 -- dfa and nfa accept the same language
 def dfa_nfa_eq : Prop := ∀ w : word σ , nfa_accepts tn w ↔ dfa_accepts td w
 
 -- to convert into nfa δ, just create singleton for each state
-def dfa_δ_to_nfa_δ : α → σ → Finset α := λ q e => {td.δ q e}
+def dfa_δ_to_nfa_δ : td.q → σ → Finset td.q := λ q e => {td.δ q e}
 
 -- conversion from nfa to dfa
-def dfa_to_nfa : NFA α σ := by
-  exact {q := td.q , init := td.init , fs := td.fs , δ := dfa_δ_to_nfa_δ td : NFA α σ}
+def dfa_to_nfa : NFA σ := by
+  exact {q := td.q , init := td.init , fs := td.fs , δ := dfa_δ_to_nfa_δ td : NFA σ}
 
 -- the initial state in NFA is same as in the original DFA
 theorem dfa_to_nfa_eq_init : td.init = (dfa_to_nfa td).init := by dsimp [dfa_to_nfa]
