lean4/Automaton/Finset/Basic.lean
@@ -1,9 +1,11 @@
 import Mathlib.Data.Finset.Basic
-
+import Mathlib.Data.Finset.Powerset
 
 namespace Finset
 
-theorem nonempty_inter_singleton_imp_in {α : Type _} [DecidableEq α] (e : α) (es : Finset α) : 
+variable {α β : Type _}
+
+theorem nonempty_inter_singleton_imp_in  [DecidableEq α] (e : α) (es : Finset α) : 
   Finset.Nonempty ({e} ∩ es) → e ∈ es := by
     intro ne
     have h₁ : e ∉ es → {e} ∩ es = ∅ := Finset.singleton_inter_of_not_mem
@@ -11,5 +13,16 @@ theorem nonempty_inter_singleton_imp_in {α : Type _} [DecidableEq α] (e : α) 
     apply h₂
     apply (Iff.mp Finset.nonempty_iff_ne_empty)
     exact ne
+
+def fin_of_subtype_to_subtype_of_subfin {qs : Finset α} (s : Finset { x // x ∈ qs }) : { x // x ⊆ Finset.attach qs } := by 
+  exact ⟨s , fun x => by simp⟩ 
+
+def subtype_of_subfin_to_fin_of_subtype {qs : Finset α}  (s : { x // x ⊆ Finset.attach qs }) : (Finset { x // x ∈ qs }) := by 
+  exact s.1
+
+def subtype_of_sset_subtype {α : Type _} {s ss : Finset α} (e : { x // x ∈ ss}) : ss ⊆ s → { x // x ∈ s} := by
+  intro iss
+  exact ⟨ e.1 , by simp; apply Finset.mem_of_subset iss; exact e.2⟩ 
+
 
 end Finset
